writing coupon

theories/examples/coupon.v
@@ -2,6 +2,7 @@
 From clutch Require Export clutch.
 From clutch.lib Require Export map.
 
+
 Set Default Proof Using "Type*".
 
 
@@ -10,10 +11,11 @@ Definition cnt_map_helper : expr :=
        if: "k" = "n"
        then #0
        else
+         let: "k'" := "k" + #1 in
          match: get "m" "k" with
-           NONE => "cnt_helper" "m" ("k"+#1) 
+           NONE => "cnt_helper" "m" "k'" "n"
          | SOME <> =>
-             #1 + "cnt_helper" "m" ("k"+#1)
+             "cnt_helper" "m" "k'" "n" + #1
          end
     ).
 
@@ -53,37 +55,191 @@ Section proofs.
   Context `{!clutchRGS Σ}.
 
   Definition couponN := nroot.@"coupon".
+  
 
-  (**  TODO! *)
-  Fixpoint cnt_gallina (vs: gmap nat val) (k:Z) (n:nat) := Z.of_nat 0.
+  Definition map_set_relate start n (m: gmap nat val) (s:gset nat)  :=
+    forall elem, elem ∈ s <-> is_Some (m !! elem) /\ start <= elem < n.
 
   (* This is an invariant in the sense that it holds true for every recursive call, 
      but we do not technically allocate it as an invariant in the RA sense. 
    *)
-  Definition coupon_collection_inv n m (k:Z) cnt cnt':= (∃(cntv : Z) lis , map_list m lis ∗ cnt' ↦ₛ #cntv ∗ cnt ↦ #cntv ∗ ⌜cnt_gallina lis 0 n = k⌝ )%I.
+  Definition coupon_collection_inv n lm (k:Z) (cnt cnt' : loc): iProp Σ :=
+    (∃(cntv : nat) s m,
+        map_list lm m ∗ ⌜map_set_relate 0 n m s⌝ ∗ cnt' ↦ₛ #cntv ∗ cnt ↦ #cntv ∗ ⌜Z.of_nat (size s) = k⌝ )%I.
 
-  Lemma coupon_collection_refines_spec_helper n m (k:Z) cnt cnt':
-    ⊢ coupon_collection_inv n m k cnt cnt' -∗ REL coupon_helper #m #n #cnt << spec_coupon_helper #k #n #cnt' : lrel_nat.
+  
+  Lemma wp_cnt_map_helper E lm m n s start:
+    start <= n ->
+    map_set_relate start n m s ->
+    {{{ map_list lm m}}}
+      cnt_map_helper #lm #start #n @ E
+      {{{v, RET #v; map_list lm m ∗ ⌜v = size s⌝}}}.
+  Proof. 
+    iIntros (H Hms Φ) "(%&%&Hlm&%&Ha) HΦ".
+    wp_pure.
+    iRevert (H H0 Hms).
+    iLöb as "IH" forall (start lv vs).
+    iIntros "%H %H0 %Hms".
+    wp_pures.
+    case_bool_decide.
+    - wp_pures. iModIntro. replace 0%Z with (Z.of_nat 0) by lia.
+      iApply ("HΦ" with "[Hlm Ha]").
+      rewrite /map_list.
+      iSplitL.
+      + iExists _, _. iFrame. by iPureIntro.
+      + subst. iPureIntro. rewrite /map_set_relate in Hms.
+        inversion H1. rewrite Nat2Z.inj_iff in H2. subst.
+        assert (s = ∅); last first.
+        { by subst. }
+        rewrite elem_of_equiv_empty_L.
+        intros. intro. rewrite Hms in H0. destruct H0 as [??].
+        lia.
+    - wp_pures. wp_bind (get _ _).
+      wp_apply (wp_get with "[Hlm Ha]").
+      { iExists _, _. iFrame. by iPureIntro. }
+      iIntros (b) "[ (%&%&Hlm&%&Ha) %Hres]".
+      subst.
+      destruct (list_to_map vs !! start) eqn:Hd.
+      + do 3 wp_pure.
+        replace (Z.of_nat start + 1)%Z with (Z.of_nat (S start)) by lia.
+        admit. 
+      + do 3 wp_pure. 
+        replace (Z.of_nat start + 1)%Z with (Z.of_nat (S start)) by lia.
+        iApply ("IH" with "[$Hlm][$Ha][$HΦ][]").
+        -- iPureIntro. destruct H; try done. lia.
+        -- by iPureIntro.
+        -- iPureIntro. intro. split; intros.
+           ++ apply Hms in H0. destruct H0. split; try done.
+              destruct H3. split; try done.
+              destruct H3; try lia. rewrite Hd in H0. inversion H0. done.
+           ++ rewrite Hms. destruct H0. split; try done.
+              destruct H3; split; try done.
+              lia.
+  Admitted.
+
+  
+
+  Lemma coupon_bijection n m s (k:Z):
+    map_set_relate 0 n m s -> Z.of_nat (size s) = k ->
+    ∃ f: (fin (S(n-1))) -> fin (S (n-1)), Bij f /\ forall x, f x < Z.to_nat k <-> is_Some (m!! fin_to_nat x).
+    Admitted. 
+
+  Lemma coupon_collection_refines_spec_helper n lm (k:Z) cnt cnt':
+    n>0->
+    ⊢ coupon_collection_inv n lm k cnt cnt' -∗ REL coupon_helper #lm #n #cnt << spec_coupon_helper #k #n #cnt' : lrel_nat.
   Proof.
+    intros.  
+    (* iLöb as "IH" forall (k). *)
+    iIntros "Inv".
+    rel_pure_l.
+    rel_pure_r.
+    iRevert "Inv".
     iLöb as "IH" forall (k).
     iIntros "Inv".
-    iDestruct "Inv" as (??) "(?&?&?&%)".
-    rewrite {2}/coupon_helper {2}/spec_coupon_helper.
-    do 10 rel_pure_l. 
+    iDestruct "Inv" as (???) "(Hml&%Hms&Hc'&Hc&%)".
+    do 9 rel_pure_l. 
     rewrite -!/cnt_map_helper.
     rel_pures_r.
     case_bool_decide.
     - (* finish collecting*)
       rel_pures_r. rel_load_r.
-      subst. 
-      inversion H0; subst. 
+      subst.
       rel_apply_l (refines_wp_l _ _ (cnt_map_helper _ _ _)).
-    Admitted. 
-  
-  Lemma coupon_collection_refines_spec:
-    ⊢ REL coupon_collection << spec_coupon_collection : lrel_nat → lrel_nat.
+      replace 0%Z with (Z.of_nat 0); last done.
+      wp_apply (wp_cnt_map_helper with "[$Hml][Hc' Hc]").
+      { lia. }
+      { done. }
+      iModIntro. iIntros (?) "[?%]". rewrite H1. rewrite H0.
+      rel_pures_l. case_bool_decide; last done.
+      rel_pures_l.
+      rel_load_l.
+      rel_values.
+    - rel_pures_r.
+      rel_load_r.
+      rel_pures_r.
+      rel_store_r.
+      rel_pures_r.
+      rel_apply_l (refines_wp_l _ _ (cnt_map_helper _ _ _)).
+      replace 0%Z with (Z.of_nat 0); last done.
+      wp_apply (wp_cnt_map_helper with "[$Hml][Hc' Hc]").
+      { lia. }
+      { done. }
+      iModIntro. iIntros (?) "[Hml %]". rewrite H2.
+      rel_pures_l.
+      case_bool_decide.
+      { rewrite H0 in H3. done. }
+      rel_pures_l.
+      rel_load_l.
+      rel_pures_l.
+      rel_store_l.
+      rel_pures_l.
+      clear H1 H2 H3. 
+      destruct (coupon_bijection _ _ _ _ Hms H0) as [f[]].
+      rel_apply (refines_couple_UU _ f).
+      { by replace (Z.to_nat (Z.of_nat n - 1)) with (n-1) by lia. }
+      iModIntro. iIntros (r).
+      rel_pures_l.
+      rel_pures_r.
+      rel_apply_l (refines_wp_l _ _ (set _ _ _)).
+      wp_apply (wp_set with "[$Hml] [Hc' Hc]").
+      iIntros "!> Hml".
+      case_bool_decide.
+      + (* new coupon *) rel_pure_r. rel_pure_l. rel_pure_l.
+        rel_pure_r. 
+        iApply ("IH" $! (k+1)%Z with "[Hc' Hc Hml]").
+        iExists _, ({[fin_to_nat r]} ∪ s), _.
+        replace (Z.of_nat cntv + 1)%Z with (Z.of_nat (S cntv)) by lia.
+        iFrame.
+        iSplit; iPureIntro.
+        -- intros. split; intros; try split.
+           ++ rewrite lookup_insert_is_Some'.
+              apply elem_of_union in H4 as [H4|H4].
+              --- rewrite elem_of_singleton in H4. subst.
+                  by left.
+              --- right. apply Hms in H4. by destruct H4.
+           ++ split; try lia.
+              apply elem_of_union in H4 as [H4|H4].
+              --- rewrite elem_of_singleton in H4. subst.
+                  replace n with (S (n-1)) by lia.
+                  apply fin_to_nat_lt.
+              --- apply Hms in H4. by destruct H4 as [?[]].
+           ++ destruct H4.
+              rewrite lookup_insert_is_Some' in H4.
+              apply elem_of_union.
+              destruct H4.
+              --- left. by apply elem_of_singleton.
+              --- right. rewrite Hms. by split.
+        -- rewrite size_union.
+           ++ rewrite size_singleton. lia.
+           ++ rewrite disjoint_singleton_l. intro. apply Hms in H4 as [??].
+              rewrite <-H2 in H4. lia. 
+      + (* old coupon *)
+        do 2 rel_pure_l.
+        rel_pure_r.
+        iApply ("IH" with "[Hc' Hc Hml]").
+        iExists _, s, _.
+        replace (Z.of_nat cntv + 1)%Z with (Z.of_nat (S cntv)) by lia.
+        iFrame.
+        iSplit; iPureIntro.
+        -- split; intros; try split.
+           ++ apply Hms in H4 as [].
+              rewrite lookup_insert_is_Some'.
+              by right.
+           ++ by apply Hms in H4 as [].
+           ++ rewrite Hms. destruct H4; split; try done.
+              rewrite lookup_insert_is_Some' in H4.
+              destruct H4.
+              --- subst. rewrite -H2.
+                  lia.
+              --- done.
+        -- done.
+ Qed. 
+    
+  Lemma coupon_collection_refines_spec n:
+    n > 0 ->
+    ⊢ REL (coupon_collection (#n)) << spec_coupon_collection (#n): lrel_nat.
   Proof.
-    rel_arrow_val. iIntros (v1 v2 [n[-> ->]]) .
+    intros.
     rel_pures_l.
     rel_pures_r.
     rel_alloc_r cnt' as "Hcnt'". do 2 rel_pure_r.
@@ -94,10 +250,15 @@ Section proofs.
     rel_alloc_l cnt as "Hcnt".
     do 2 rel_pure_l.
     rewrite -/coupon_helper -/spec_coupon_helper.
-    iApply (coupon_collection_refines_spec_helper with "[Hcnt' Hm Hcnt]").
-    rewrite /coupon_collection_inv; iExists _, _. iFrame.
-    by iPureIntro. 
-Qed. 
+    iApply (coupon_collection_refines_spec_helper with "[Hcnt' Hm Hcnt]"); [done|].
+    rewrite /coupon_collection_inv. iExists 0, ∅. iFrame.
+    iExists _. iFrame.
+    iSplit.
+    - iPureIntro. intros. split; intros; [by rewrite elem_of_empty in H0|]. 
+      destruct H0 as [H' ?]. rewrite lookup_empty in H'. destruct H' as [H'?].
+      inversion H1. 
+    - iPureIntro. done. 
+  Qed. 
 
   
   
